Start fixing the proofs in SimplifyEmptyBlocks

src/Passes/SimplifyEmptyBlocks.dfy
@@ -7,6 +7,7 @@ include "../Utils/StrTree.dfy"
 include "../Semantics/Interp.dfy"
 include "../Semantics/Equiv.dfy"
 include "../Semantics/Pure.dfy"
+include "../Semantics/EqInterpRefl.dfy"
 include "../Transforms/BottomUp.dfy"
 include "EliminateNegatedBinops.dfy"
 
@@ -288,15 +289,29 @@ module FilterEmptyBlocks {
           reveal InterpExpr();
           reveal InterpBlock();
 
-          var ctx1 := ctx.(rollback := map []);
-          var ctx1' := ctx'.(rollback := map []);
+          var ctx1 := StartScope(ctx);
+          var ctx1' := StartScope(ctx');
 
           assert EqState(ctx1, ctx1') by {
             reveal GEqCtx();
           }
 
           FilterEmptyBlocks_Seq_Rel(es, env, ctx1, ctx1');
-          reveal GEqCtx();
+          var res2 := InterpBlock_Exprs(es, env, ctx1);
+          var res2' := InterpBlock_Exprs(FilterEmptyBlocks_Seq(es), env, ctx1');
+          assert EqInterpResultValue(res2, res2');
+
+          if res2.Success? {
+            var Return(v, ctx2) := res2.value;
+            var Return(v', ctx2') := res2'.value;
+            assert EqValue(v, v');
+            assert EqState(ctx2, ctx2');
+
+            var ctx3 := EndScope(ctx, ctx2);
+            var ctx3' := EndScope(ctx', ctx2');
+            assert EqState(ctx3, ctx3') by { reveal GEqCtx(); }
+          }
+          else {}
       }
 
       assert SupportsInterp(e');
@@ -321,6 +336,7 @@ module InlineLastBlock {
   import opened Semantics.Interp
   import opened Semantics.Values
   import opened Semantics.Equiv
+  import opened Semantics.EqInterpRefl
   import opened Transforms.Generic
   import opened Transforms.Proofs.BottomUp_
 
@@ -359,11 +375,26 @@ module InlineLastBlock {
     else e
   }
 
+  // TODO(SMH): remove this definition once GEqState is updated
+  predicate EqInterpResultValueRollback(res: InterpResult<Interp.Value>, res': InterpResult<Interp.Value>)
+  {
+    match (res, res') {
+      case (Success(Return(v, ctx)), Success(Return(v', ctx'))) =>
+        && EqCtx(ctx.locals, ctx'.locals)
+        && EqCtx(ctx.locals + ctx.rollback, ctx'.locals + ctx'.rollback)
+        && EqValue(v, v')
+      case (Failure(_), _) =>
+        true
+      case _ =>
+        false
+    }
+  }
+  
   lemma InlineLastBlock_Seq_Rel(es: seq<Expr>, env: Environment, ctx: State, ctx': State)
     requires forall e | e in es :: SupportsInterp(e)
     requires EqState(ctx, ctx')
     ensures forall e | e in InlineLastBlock_Seq(es) :: SupportsInterp(e)
-    ensures EqInterpResultValue(InterpBlock_Exprs(es, env, ctx), InterpBlock_Exprs(InlineLastBlock_Seq(es), env, ctx'))
+    ensures EqInterpResultValueRollback(InterpBlock_Exprs(es, env, ctx), InterpBlock_Exprs(InlineLastBlock_Seq(es), env, ctx'))
   {
     reveal InterpBlock_Exprs();
 
@@ -384,20 +415,20 @@ module InlineLastBlock {
         assert res == InterpExpr(es[0], env, ctx);
         assert InterpExpr(es[0], env, ctx) == InterpBlock(es[0].stmts, env, ctx);
 
-        var ctx1 := ctx.(rollback := map []);
-        var ctx1' := ctx'.(rollback := map []);
+        var ctx1 := StartScope(ctx);
+        var ctx1' := StartScope(ctx');
         assert EqState(ctx1, ctx1') by {
           reveal GEqCtx();
         }
 
-        assume TODO(); // TODO: fix proof
-
         assert es' == es[0].stmts;
-        InterpBlock_Exprs_Refl(es[0].stmts, env, ctx, ctx');
+
+        assume TODO(); // TODO: fix proof
       }
       else {
         assert es == es';
-        InterpBlock_Exprs_Refl(es, env, ctx, ctx');
+        assert Seq_All(SupportsInterp, es);
+        InterpBlock_Exprs_EqRefl(es, env, ctx, ctx');
       }
     }
     else {
@@ -410,10 +441,11 @@ module InlineLastBlock {
       var tl' := InlineLastBlock_Seq(tl);
 
       forall env, ctx, ctx' | EqState(ctx, ctx')
-        ensures EqInterpResultValue(InterpBlock_Exprs(tl, env, ctx), InterpBlock_Exprs(tl', env, ctx'))
+        ensures EqInterpResultValueRollback(InterpBlock_Exprs(tl, env, ctx), InterpBlock_Exprs(tl', env, ctx'))
       {
         InlineLastBlock_Seq_Rel(tl, env, ctx, ctx');
       }
+      assume false; // TODO: fix
       InterpBlock_Exprs_Eq_Append(es[0], es[0], tl, tl', env, ctx, ctx');
     }
   }
@@ -435,8 +467,8 @@ module InlineLastBlock {
         reveal InterpExpr();
         reveal InterpBlock();
 
-        var ctx1 := ctx.(rollback := map []);
-        var ctx1' := ctx'.(rollback := map []);
+        var ctx1 := StartScope(ctx);
+        var ctx1' := StartScope(ctx');
 
         assert EqState(ctx1, ctx1') by {
           reveal GEqCtx();
