src/Semantics/EqInterpRefl.dfy
@@ -1,0 +1,412 @@
+include "../Interop/CSharpDafnyASTModel.dfy"
+include "../Interop/CSharpInterop.dfy"
+include "../Interop/CSharpDafnyInterop.dfy"
+include "../Interop/CSharpDafnyASTInterop.dfy"
+include "../Utils/Library.dfy"
+include "../Utils/StrTree.dfy"
+include "Interp.dfy"
+include "Equiv.dfy"
+include "ExprInduction.dfy"
+
+module Bootstrap.Semantics.EqInterpRefl {
+
+module Base refines ExprInduction.Ind {
+  //
+  // Declarations
+  //
+  type Value = Interp.Value
+
+  datatype MState = MState(env: Environment, ctx: State, ctx': State)
+  datatype MValue = MValue(v: Value, v': Value)
+  datatype MSeqValue = MSeqValue(vs: seq<Value>, vs': seq<Value>)
+
+  type S(!new) = MState
+  type V(!new) = MValue
+  type VS(!new) = vs:MSeqValue | |vs.vs| == |vs.vs'| witness MSeqValue([], [])
+
+  predicate P(st: S, e: Expr)
+  {
+    EqState(st.ctx, st.ctx') ==>
+    EqInterpResultValue(InterpExpr(e, st.env, st.ctx), InterpExpr(e, st.env, st.ctx'))
+  }
+  
+  predicate P_Succ(st: S, e: Expr, st': S, v: V)
+  {
+    && EqState(st.ctx, st.ctx')
+    && EqInterpResultValue(InterpExpr(e, st.env, st.ctx), InterpExpr(e, st.env, st.ctx'))
+    && InterpExpr(e, st.env, st.ctx) == Success(Return(v.v, st'.ctx))
+    && InterpExpr(e, st.env, st.ctx') == Success(Return(v.v', st'.ctx'))
+    && st.env == st'.env
+  }
+
+  predicate P_Fail(st: S, e: Expr)
+  {
+    EqState(st.ctx, st.ctx') ==> InterpExpr(e, st.env, st.ctx).Failure?
+  }
+
+  predicate Pes(st: S, es: seq<Expr>)
+  {
+    EqState(st.ctx, st.ctx') ==>
+    EqInterpResultSeqValue(InterpExprs(es, st.env, st.ctx), InterpExprs(es, st.env, st.ctx'))
+  }
+
+  predicate Pes_Succ(st: S, es: seq<Expr>, st': S, vs: VS)
+  {
+    && EqState(st.ctx, st.ctx')
+    && EqInterpResultSeqValue(InterpExprs(es, st.env, st.ctx), InterpExprs(es, st.env, st.ctx'))
+    && InterpExprs(es, st.env, st.ctx) == Success(Return(vs.vs, st'.ctx))
+    && InterpExprs(es, st.env, st.ctx') == Success(Return(vs.vs', st'.ctx'))
+    && st.env == st'.env
+  }
+
+  predicate Pes_Fail(st: S, es: seq<Expr>)
+  {
+    !EqState(st.ctx, st.ctx') || InterpExprs(es, st.env, st.ctx).Failure?
+  }
+
+  function AppendValue ...
+  {
+    MSeqValue([v.v] + vs.vs, [v.v'] + vs.vs')
+  }
+
+  function SeqVToVS ...
+  {
+    if vs == [] then MSeqValue([], [])
+    else
+      AppendValue(MValue(vs[0].v, vs[0].v'), SeqVToVS(vs[1..]))
+  }
+  
+  function GetNilVS ...
+  {
+    MSeqValue([], [])
+  }
+
+  ghost const UnitV := MValue(Values.Unit, Values.Unit)
+
+  function VS_Last ...
+  {
+    var v := vs.vs[|vs.vs| - 1];
+    var v' := vs.vs'[|vs.vs| - 1];
+    MValue(v, v')
+  }
+
+  predicate VS_UpdateStatePre ...
+  {
+    && |argvs.vs| == |argvs.vs'| == |vars|
+    && forall i | 0 <= i < |argvs.vs| :: EqValue(argvs.vs[i], argvs.vs'[i])
+  }
+
+  function BuildClosureCallState ...
+    // Adding this precondition makes the InductAbs proofs easier
+    ensures
+      EqState(st.ctx, st.ctx') ==>
+      EqState(st'.ctx, st'.ctx')
+  {
+    var ctx1 := BuildCallState(st.ctx.locals, vars, argvs.vs);
+    var ctx1' := BuildCallState(st.ctx'.locals, vars, argvs.vs');
+    var st' := MState(env, ctx1, ctx1');
+    assert EqState(st.ctx, st.ctx') ==> EqState(st'.ctx, st'.ctx') by {
+      if EqState(st.ctx, st.ctx') {
+        BuildCallState_EqState(st.ctx.locals, st.ctx'.locals, vars, argvs.vs, argvs.vs');
+      }
+    }
+    st'
+  }
+
+  function UpdateState ...
+    // Adding this precondition makes the InductUpdate proofs easier
+    ensures
+      EqState(st.ctx, st.ctx') ==>
+      EqState(st'.ctx, st'.ctx')
+  {
+    var ctx1 := st.ctx.(locals := AugmentContext(st.ctx.locals, vars, vals.vs));
+    var ctx1' := st.ctx'.(locals := AugmentContext(st.ctx'.locals, vars, vals.vs'));
+    var st' := MState(st.env, ctx1, ctx1');
+
+    reveal BuildCallState();
+    assert EqState(st.ctx, st.ctx') ==> EqState(st'.ctx, st'.ctx') by {
+      if EqState(st.ctx, st.ctx') {
+        BuildCallState_EqState(st.ctx.locals, st.ctx'.locals, vars, vals.vs, vals.vs');
+      }
+    }
+
+    st'
+  }
+
+  function StateSaveToRollback ...
+    ensures EqState(st.ctx, st.ctx') ==> EqState(st'.ctx, st'.ctx')
+  {
+    var ctx := SaveToRollback(st.ctx, vars);
+    var ctx' := SaveToRollback(st.ctx', vars);
+    var st' := MState(st.env, ctx, ctx');
+
+    reveal GEqCtx();
+    assert EqState(st.ctx, st.ctx') ==> EqState(st'.ctx, st'.ctx') by {
+      if EqState(st.ctx, st.ctx') {
+        SaveToRollback_Equiv(st.ctx, st.ctx', vars);
+      }
+    }
+
+    st'
+  }
+
+  function StateStartScope ...
+    ensures EqState(st.ctx, st.ctx') ==> EqState(st'.ctx, st'.ctx')
+  {
+    var ctx := StartScope(st.ctx);
+    var ctx' := StartScope(st.ctx');
+    reveal GEqCtx();
+    MState(st.env, ctx, ctx')
+  }
+
+  function StateEndScope ...
+    ensures EqState(st0.ctx, st0.ctx') && EqState(st.ctx, st.ctx') ==> EqState(st'.ctx, st'.ctx')
+  {
+    var ctx := EndScope(st0.ctx, st.ctx);
+    var ctx' := EndScope(st0.ctx', st.ctx');
+    reveal GEqCtx();
+    MState(st.env, ctx, ctx')
+  }
+
+  function P_Step ... {
+    var Return(v, ctx1) := InterpExpr(e, st.env, st.ctx).value;
+    var Return(v', ctx1') := InterpExpr(e, st.env, st.ctx').value;
+    (MState(st.env, ctx1, ctx1'), MValue(v, v'))
+  }
+
+  function Pes_Step ... {
+    var Return(vs, ctx1) := InterpExprs(es, st.env, st.ctx).value;
+    var Return(vs', ctx1') := InterpExprs(es, st.env, st.ctx').value;
+    (MState(st.env, ctx1, ctx1'), MSeqValue(vs, vs'))
+  }
+
+  //
+  // Lemmas
+  //
+
+  lemma P_Fail_Sound ... {}
+  lemma P_Succ_Sound ... {}
+  lemma Pes_Fail_Sound ... {}
+  lemma Pes_Succ_Sound ... {}
+
+  lemma Pes_Succ_Inj ... {}
+  lemma SeqVToVS_Append ... {}
+
+  lemma InductVar ... {
+    reveal InterpExpr();
+    reveal GEqCtx();
+
+    var env := st.env;
+    var v := e.name;
+    
+    // Start by looking in the local context
+    var res0 := TryGetVariable(st.ctx.locals, v, UnboundVariable(v));
+    var res0' := TryGetVariable(st.ctx'.locals, v, UnboundVariable(v));
+
+    if res0.Success? {
+      assert res0.Success?;
+    }
+    else {
+      // Not in the local context: look in the global context
+      assert v in env.globals;
+      EqValue_Refl(env.globals[v]);
+    }
+  }
+
+  lemma InductLiteral ... { reveal InterpExpr(); reveal InterpLiteral(); }
+
+  lemma InductAbs ... {
+    reveal InterpExpr();
+    reveal EqValue_Closure();
+
+    var MState(env, ctx, ctx') := st;
+    var cv := Values.Closure(ctx.locals, vars, body);
+    var cv' := Values.Closure(ctx'.locals, vars, body);
+
+    forall env, argvs, argvs' |
+      && |argvs| == |argvs'| == |vars|
+      && (forall i | 0 <= i < |vars| :: EqValue(argvs[i], argvs'[i]))
+      ensures
+        var res := InterpCallFunctionBody(cv, env, argvs);
+        var res' := InterpCallFunctionBody(cv', env, argvs');
+        EqPureInterpResultValue(res, res')
+    {
+      // The following triggers instantiations
+      var argvs := MSeqValue(argvs, argvs');
+      assert P(BuildClosureCallState(st, vars, body, env, argvs), body);
+
+      reveal InterpCallFunctionBody();
+    }
+
+    assert EqValue_Closure(cv, cv');
+  }
+
+  lemma InductAbs_CallState ... {
+    reveal InterpExpr();
+    reveal InterpCallFunctionBody();
+    reveal BuildCallState();
+  }
+
+  lemma InductExprs_Nil ... { reveal InterpExprs(); }
+  lemma InductExprs_Cons ... { reveal InterpExprs(); }
+
+  lemma InductApplyLazy_Fail ... { reveal InterpExpr(); reveal InterpLazy(); }
+  lemma InductApplyLazy_Succ ... { reveal InterpExpr(); reveal InterpLazy(); }
+
+  lemma InductApplyEager_Fail ... { reveal InterpExpr(); }
+
+  lemma InductApplyEagerUnaryOp_Succ ... { reveal InterpExpr(); reveal InterpUnaryOp(); }
+
+  lemma InductApplyEagerBinaryOp_Succ ... {
+    reveal InterpExpr();
+    InterpBinaryOp_Eq(e, e, op, v0.v, v1.v, v0.v', v1.v');
+  }
+
+  lemma InductApplyEagerTernaryOp_Succ ... {
+    reveal InterpExpr();
+    reveal InterpTernaryOp();
+
+    // TODO: using this lemma makes Dafny crash:
+    // InterpTernaryOp_Eq(e, e, op, v0.v, v1.v, v2.v, v0.v', v1.v', v2.v');
+
+    EqValue_HasEqValue_Eq(v0.v, v0.v');
+    EqValue_HasEqValue_Eq(v1.v, v1.v');
+  }
+
+  lemma InductApplyEagerBuiltinDisplay ... {
+    reveal InterpExpr();
+    Interp_Apply_Display_EqValue(e, e, ty.kind, argvs.vs, argvs.vs');
+  }
+
+  lemma InductApplyEagerFunctionCall ... {
+    reveal InterpExpr();
+    InterpFunctionCall_EqState(e, e, st.env, fv.v, fv.v', argvs.vs, argvs.vs');
+  }
+
+  lemma InductIf_Fail ... { reveal InterpExpr(); }
+  lemma InductIf_Succ ... { reveal InterpExpr(); }
+
+  lemma InductUpdate_Fail ... { reveal InterpExpr(); }
+  lemma InductUpdate_Succ ... { reveal InterpExpr(); }
+
+  lemma InductVarDecl_None_Succ ... { reveal InterpExpr(); }
+  lemma InductVarDecl_Some_Fail ... { reveal InterpExpr(); }
+  lemma InductVarDecl_Some_Succ  ... { reveal InterpExpr(); }
+
+  // TODO(SMH): I tried simplifying the proofs below by adding a `requires` in ``InductBlock_Fail``
+  // and ``InductBlock_Succ`` to provide the assertions and the results of calling the lemmas used
+  // in the proof below, but it didn't work due to SMT solvers' misteries.
+  lemma InductBlock_Fail ...
+  {
+    reveal InterpExpr();
+    reveal InterpBlock();
+    reveal InterpExprs();
+    reveal InterpBlock_Exprs();
+    reveal InterpExprs_Block();
+
+    var env := st.env;
+
+    // We need this because of the fuel
+    assert InterpExpr(e, env, st.ctx) == InterpBlock(stmts, env, st.ctx);
+    assert InterpExpr(e, env, st.ctx') == InterpBlock(stmts, env, st.ctx');
+    
+    InterpExprs_Block_Equiv_Strong(stmts, env, st_start.ctx);
+    InterpExprs_Block_Equiv_Strong(stmts, env, st_start.ctx');
+  }
+
+  lemma InductBlock_Succ ...
+  {
+    reveal InterpExpr();
+    reveal InterpBlock();
+    reveal InterpExprs();
+    reveal InterpBlock_Exprs();
+    reveal InterpExprs_Block();
+
+    var env := st.env;
+
+    // We need this because of the fuel
+    assert InterpExpr(e, env, st.ctx) == InterpBlock(stmts, env, st.ctx);
+    assert InterpExpr(e, env, st.ctx') == InterpBlock(stmts, env, st.ctx');
+    
+    InterpExprs_Block_Equiv_Strong(stmts, env, st_start.ctx);
+    InterpExprs_Block_Equiv_Strong(stmts, env, st_start.ctx');
+  }
+
+} // end of module Bootstrap.Semantics.EqInterpRefl.Base
+
+  import opened AST.Syntax
+  import opened Utils.Lib
+  import opened AST.Predicates
+  import opened Interp
+  import opened Values
+  import opened Equiv
+  import opened Utils.Lib.Datatypes
+  import opened Base
+
+  type Expr = Interp.Expr
+
+  lemma InterpBlock_Exprs_EqRefl(es: seq<Expr>, env: Environment, ctx: State, ctx': State)
+    // TODO(SMH): for some reason, using ``Seq_All`` makes some proofs fail. The weird thing is
+    // that I can then prove `Seq_All(SupportsInterp, es)` in an assertion just before the call
+    // to the lemma, but the lemma precondition keeps failing.
+    requires forall e | e in es :: SupportsInterp(e)
+    requires EqState(ctx, ctx')
+    ensures EqInterpResultValue(InterpBlock_Exprs(es, env, ctx), InterpBlock_Exprs(es, env, ctx'))
+  {
+    InterpExprs_Block_Equiv_Strong(es, env, ctx);
+    InterpExprs_Block_Equiv_Strong(es, env, ctx');
+    Base.Pes_Satisfied(MState(env, ctx, ctx'), es);
+
+    reveal InterpExprs_Block();
+  }
+
+  lemma InterpExprs_EqRefl(es: seq<Expr>, env: Environment, ctx: State, ctx': State)
+    requires EqState(ctx, ctx')
+    ensures EqInterpResultSeqValue(InterpExprs(es, env, ctx), InterpExprs(es, env, ctx'))
+  {
+    Base.Pes_Satisfied(MState(env, ctx, ctx'), es);
+  }
+
+  // DISCUSS: the proof actually indirectly relies on the fact that ``EqValue`` is reflexive.
+  // But the proof that ``EqValue`` is reflexive (not done) relies, for the closure case, on the fact
+  // that ``InterpExpr`` is reflexive. The termination argument is not trivial, and we may have to
+  // rely on step-indexing.
+  //
+  // Here is an old comment, which gives some insight about what is going on:
+  //
+  // Actually the proof of termination is an issue in the case we lookup a global
+  // variable, because the global environment always stays the same...
+  //
+  // I think we could do the proof as follows:
+  // - define an EqValueN relation which is parameterized by a fuel (which is used for
+  //   the closures - and thus not quantified in EqValue_Closure)
+  // - for the closures, the EqValue applied on the returned results would use the fuel
+  //   remaining after the bodies have been executed (this would solve the problem of
+  //   proving reflexivity about the values in the environment, when looking up globals,
+  //   in particular)
+  // - prove the reflexivity for EqValueN: forall v n. EqValueN(v, v, n)
+  // - from this theorem, we should be able to prove the reflexivity theorem. The tricky
+  //   case is for closures, in which case we should use the fact that:
+  //
+  //   forall fuel fuel' ::
+  //     var res := Interp(..., fuel);
+  //     var res' := Interp(..., fuel');
+  //     res.Success? ==>
+  //       fuel' >= fuel - res.ctx.fuel ==>
+  //         res'.Success? && res'.ctx.fuel == fuel' - (fuel - res.ctx.fuel)
+  //
+  //   This way, we would be able to properly instantiate the initial fuel to get:
+  //   
+  //   forall n. EqInterpResultValueN(..., n)
+  //
+  //   Finally, we would get: EqInterpResultValue(...) by using the induction hypothesis
+  //   (where termination is given by the fact that the type of the return value is smaller
+  //   than the type of the closure).
+  lemma InterpExpr_EqRefl(e: Expr, env: Environment, ctx: State, ctx': State)
+    requires EqState(ctx, ctx')
+    ensures EqInterpResultValue(InterpExpr(e, env, ctx), InterpExpr(e, env, ctx'))
+  {
+    Base.P_Satisfied(MState(env, ctx, ctx'), e);
+  }
+
+} // end of module Bootstrap.Semantics.EqInterpRefl
